test-suite/evars.v
@@ -1,0 +1,13 @@
+Require Import Template.Template.
+
+Goal True.
+  evar (n : nat).
+  match goal with
+    H := ?t |- _ => quote_term t (fun x => pose (qn:=x))
+  end.
+  match goal with
+    qn := Ast.tEvar _ nil |- _ => idtac
+  end.
+  exact I.
+  Unshelve. exact 0.
+Qed.
